---
title: "Task Solution Chapter 3"
author: "Witold Wolski"
date: "December 3, 2016"
output:
  html_document: default
  pdf_document: default
---

```{r setup, include=FALSE}
knitr::opts_chunk$set(echo = TRUE)
```

## Task 1

Verify formula for $var(Y)$

$$
var(Y) = \frac{\phi}{w} b''(\theta)
$$


$$
l(\theta, \phi, y) = \frac{y\theta- b(\theta)}{\phi/w} + c(y,\phi)
$$

and using proofs in 3.3.2.

To warm up lets show that the mean is equal to $b'(\theta)$. 

$$
\begin{aligned}
0 &= E(\frac{\partial l}{ \partial \theta})\\
&= E(\frac{y-b'(\theta)}{\phi / w}) = w/\phi E(y-b'(\theta)) = w/\phi(E(y) - b'(\theta))\\
&\rightarrow E(Y) =  b'(\theta)
\end{aligned}
$$


According to Result 2 on page 64 

with:


$$
\begin{aligned}
-E(\frac{\partial^2 l }{\partial \theta^2}) &= E(\frac{\partial l}{\partial \theta}^2)\\
-E(-wb''(\theta)/\phi) &= E((\frac{y-b'(\theta)}{\phi / w})^2)\\
w/\phi E(b''(\theta))  &= (w/\phi)^2 E((y-E(Y))^2)\\
\phi/w E(b''(\theta)) &= E((y-E(Y))^2)\\
\frac{\phi}{w} b''(\theta) &= Var(Y)
\end{aligned}
$$

with $Var(Y) = E((y-E(Y))^2)$ and $E(b''(\theta)) = b''(\theta)$ (but this seems quite a stretch). 


## Task 2

Use equations (3.8) and (3.9) to verify the entries in the table above.

Equation (3.8) is:
$$
\mu = E(Y) = b'(\theta)
$$

Equation (3.9) is:

$$
var(Y) = \frac{\phi}{w} b''(\theta)
$$

### i

For normal distribution:
$$
b(\theta) = \theta^2/2 \rightarrow b'(\theta) = \theta \rightarrow b''(\theta) = 1
$$

### ii

For Poisson distribution

$$
b(\theta) = e^\theta \rightarrow b'(\theta) = e^\theta \rightarrow b''(\theta) = e^\theta
$$

### iii
For Binomial



$$
b(\theta)  = \log(1 + e^\theta) \rightarrow b'(\theta) = \frac{e^\theta}{1+e^\theta} 
\rightarrow b''(\theta) = \frac{e^\theta}{e^\theta + 1} - \frac{e^{2\theta}}{(e^\theta + 1)^2}
$$

Need to check how to differentiate this.

### iv

For Gamma
$$
b(\theta) = -log(-\theta) \rightarrow b'(\theta) = +1/\theta \rightarrow b''(\theta) = 1/\theta^2 =
(-1\theta)^2 = \mu^2
$$




# Task 3

Task 3 Verify the canonical links for the Normal, Binomial, Poisson and Gamma.

The link function $g$ for which $\theta_i = x^T_i\beta$
(that is, for which $g = (b')^{-1}$) is called the canonical link.

Hence, the task is to find the inverse of $g=(b')^{-1}$.

### for Normal
$$
b'(\theta) = \theta \rightarrow \theta = g(\mu) = 1(\mu)
$$

### for Poisson

$$
b'(\theta) = e^\theta \rightarrow \mu = e^\theta \rightarrow \theta = \log(\mu)
$$

### for Binomial

$$
b'(\theta) = \log(1+e^\theta) \rightarrow \mu = \log(1+e^\theta) \rightarrow \theta =  \log(\mu_i /(1 - \mu_i ))
$$


### For Gamma

$$
b'(\theta) = -1/\theta \rightarrow \mu = -1/\theta \rightarrow \theta = g(\mu) = -1/\mu
$$


# Task 4

For the canonical link (see, in particular, equation (3.10)) show that


$$
\begin{aligned}
\frac{\partial^2 l}{\partial \beta_j \partial \beta_k} &= \frac{1}{\phi} \frac{\partial^2 l}{\partial \beta_j \partial \beta_k}(\sum_i \{w_i[y_i\theta_i - b(\theta_i)] \}) \\
&= \frac{1}{\phi} \sum_i w_i \frac{\partial^2 l}{\partial \beta_j \partial \beta_k}\{[y_i\theta_i - b(\theta_i)] \}
\end{aligned}

$$

$$
\frac{\partial^2 y_i\theta_i}{\partial \beta_j \partial \beta_k} =  \frac{\partial^2 y_ix_i^T\beta}{\partial \beta_j \partial \beta_k} = 0
$$

$$
\frac{\partial^2 b(\theta_i)}{\partial \beta_j \partial \beta_k} =  \frac{\partial^2 b(\theta_i)}{\partial \theta_i^2}\frac{\partial^2 x_i^T \beta}{\partial \beta_j}\frac{\partial^2 x_i^T \beta}{\partial \beta_k} + 0 = b''(x_i^T\beta)x_{ij}x_{ik} = h'(x_i^T\beta)x_{ij}x_{ik}
$$
with chain rule of differentiation and $b'(x_i^T \beta) = h(x_i^T\beta)$.

Plugging this into Equation 1:

$$
\frac{\partial^2 l}{\partial \beta_j \partial \beta_k} &= \frac{1}{\phi} \sum_i \{-x_{ij}w_ih'(x^T_i\beta)x_{ik}\}

$$

# Task 5

Show that, for the maximal model, $y_i$ is the maximum likelihood estimate of $\mu_i$. 
(Hint: the likelihood equation for $\theta_i$ is $y_i = b'(\theta_i)$, and we already know that $b'(\theta_i) = \mu_i$ .)



$$
y_i = b'(\theta_i) = \mu_i
$$


$$
l(\mu;y,\phi) = \sum_i{\frac{y_i\theta - b(\theta)}{\phi/w_i}} + c(y,\phi)
$$

For the maximal model :

$$
\begin{aligned}
\partial l / \partial \theta_i &= (w_i /\phi) \{y_i - b'(\theta_i)\} = 0\\
\rightarrow y_i &= b'(\theta_i) = \mu_i
\end{aligned}
$$

for other models:

$$
\partial l / \partial \theta_i = \sum_i (w_i /\phi) \{y_i - b'(\theta_i)\} = 0
$$

<!---->

The model that allows the mean of each observation to be a separate parameter is called the
__full__, __saturated__ or __maximal__ model.

The maximum possible value of $L$ as the components of $\mu$ vary without any restrictions (or, essentially equivalently, when there is an element of $\beta$ for each observation, so that $\mu^\diamond_i  = h(\eta i ) = h(\beta i )$ occurs when $\mu^\diamond_i = y_i$, hence $\mu^\diamond_i = y_i$ for all $i$.


# Task 6

Deviances for common distributions.

Confirm results using the table in 3.3.4 and equation (3.12).

Eq $3.12$ is:

$$
D(y,\hat{\mu}) = \phi S(y,\hat{\mu}) = 2 \sum_i w_i [y_i(\hat{\theta^\diamond_i} - \hat{\theta_i}) - 
b(\hat{\theta^\diamond_i}) + b(\hat{\theta_i})]
$$

### For Normal

$\hat{\theta^\diamond} = y_i$ and $\hat{\theta} = \mu$; $b(\theta) = \theta^2/2$ than
$b(\hat{\theta^\diamond}) = y_i^2/2$ and $b(\hat{\theta}) = \mu^2/2$; and $w_i = 1$.


$$
\begin{aligned}
2 \sum_i  [y_i(y_i -\mu) -  y_i^2/2 + \mu^2/2]\\
&= 2 \sum_i  [y_i^2 - y_i\mu -  y_i^2/2 + \mu^2/2]\\
&=  \sum_i  [y_i^2 - 2y_i\mu+ \mu^2]\\
&= \sum_i (y_i - \mu)^2
\end{aligned}
$$

### For Poisson

$\mu = e^\theta \rightarrow \theta=\log(\mu)$.
Than

$\hat{\theta} = \log(\mu)$ and $\hat{\theta^\diamond} = \log{y_i}$; $b(\theta) = e^\theta$ than


$b(\hat{\theta^\diamond}) = e^{\log(y_i)} = y_i$ and $b(\hat{\theta}) = e^{\log(\mu)} = \mu$ and
$\phi = 1$, $w_i = 1$


$$
2\sum_i\{ y_i(\log(y_i) - \log(\mu)) - y_i + \mu \} = 2\sum_i\{ y_i\log(y_i/\mu) - y_i + \mu \}
$$

## For Binomial

TODO


# Task 7

Use the results in 3.6.4 to obtain simple expressions for the null deviance for Poisson
(weights must be one) and Gamma (assume weights are one).

If $W = \sum w_i$
$$
\mu = \sum w_i y_i / W
$$

For Poisson and Gamma model $w_i =1$, than $\mu = 1/N \sum y_i$

### For Poison

$$
\begin{aligned}
2\sum y_i \log(y_i/\hat{\mu}_i) - (y_i - \hat{\mu}_i) &=\\ 
&= 2\sum (y_i \log(\frac{y_i}{1/N \sum y_i}) - (y_i - 1/N \sum y_i)) \\
&= 2\sum (y_i \log(y_i) - \log(1/N \sum y_i) - (y_i) + (1/N \sum y_i))\\
&=2\sum y_i (\log(y_i) - \log(1/N \sum y_i))
\end{aligned}
$$

### For Gamma

Similarly, TODO

# Task 8

For the Poisson distribution, verify that $D$ and $\chi^2$ are asymptotically equivalent. (Hint:
use that for small $|x - y|, x\log(x/y) \approx (x - y) + (x - y)^2 /(2y)$.)

$$
\chi^2 = \sum e^2_{P,i} = \sum (\sqrt{w_i} \frac{y_i - \hat{\mu}_i}{\sqrt{V(\hat{\mu}_i)}})^2
$$

for Poisson $w_i = 1$ and $Var(Y_i) = \frac{\phi}{w_i}V(\mu_i) = \frac{\phi}{w_i}b''(\theta)$ and 
$b''(\theta) = V(\mu_i) = \mu$,

than:

$$
\chi^2 = \sum e^2_{P,i} = \sum (\frac{y_i - \hat{\mu}_i}{\sqrt{\mu_i}})^2
$$

$$
\begin{aligned}
D(y_i,\mu_i)=2\sum y_i \log(y_i/\hat{\mu}_i) - (y_i - \hat{\mu}_i) &=\\
&= 2\sum (y_i - \hat{\mu}_i) + (y_i - \hat{\mu}_i)^2 /(2\hat{\mu_i}) - (y_i - \hat{\mu}_i) &=\\
&= \sum((y_i - \hat{\mu}_i)^2 /\hat{\mu_i})
\end{aligned}
$$


<!--2\sum y_i \log(y_i/\hat{\mu}_i) - (y_i - \hat{\mu}_i) -->

# Task 9

Obtain the form of the __Pearson residual__ for the Binomial, Poisson and Gamma. (These
are given in Chapters 4 and 5)

$$
e_{P,i} = w_i\frac{y_i - \hat{y_i}}{\sqrt{V(\hat{\mu_i)}}} \\
$$


### For Binomial

$$
Var(\mu_i) =  \phi/w_i b''(\theta) = (1/n) \mu(1-\mu)
$$

than

$$
e_{p,i} = \frac{y_i - \mu_i}{Var(\mu_i)} \stackrel{with 1}{=} \frac{y_i - \mu_i}{\sqrt{\mu_i(1-\mu_i)/n_i}}
$$

### For Poisson

$$
Var(\mu_i) = \phi/w_i b''(\theta) = (1/1) \mu
$$

than

$$
e_{p,i} = \frac{y_i - \mu_i}{\sqrt{\mu_i}}
$$


### For Gamma

$$
Var(\mu_i) = \phi/w_i b''(\theta) = (\phi/1) \mu^2
$$

than

$$
e_{p,i} = \frac{y_i - \mu_i}{\sqrt{\phi} \mu_i}
$$


# Task 10 

- How does a GLM with identity link relate to a linear model?

It's the same as a linear model.

- Under which situations does it make sense to fit a linear model instead of a GLM with identity link?

Almost always when the response $y$ is continuous and normally distributed. 


# Task 11

Confirm that:

$$
\chi^2 = \sum e^2_{P,i} = \sum\{ \frac{[s_i -n_i \hat{\mu_i}]^2}{n_i\hat{\mu_i}} + \frac{[(n_i-s_i) - n_i (1-\hat{\mu_i})]^2}{n_i(1-\hat{\mu_i)}}\}
$$

with

$$
e_{P,i} = \frac{y_i - \hat{\mu_i}}{\sqrt{\hat{\mu_i}(1-\hat{\mu_i})/n_i}}
$$

and $s_i = n_iy_i$.

use:

$$
\frac{1}{p(1-p)} = \frac{1}{p} + \frac{1}{1-p}
$$

